examples/cannon2/HCannon0.v
@@ -1,0 +1,42 @@
+Require Import Coqlib.
+Require Import ImpPrelude.
+Require Import STS.
+Require Import Behavior.
+Require Import ModSem.
+Require Import Skeleton.
+Require Import PCM.
+Require Import HoareDef.
+Set Implicit Arguments.
+
+
+
+
+
+
+Section CANNON.
+  Context `{Σ: GRA.t}.
+  Definition div (n m: Z): option Z :=
+    if Z_zerop m then None else Some (Z.div n m).
+
+  Definition fire_body {E} `{hAGE -< E} `{callE -< E} `{sE -< E} `{eventE -< E}
+    : list val -> itree E Z :=
+    fun args =>
+      powder <- trigger sGet;; powder <- powder↓?;;
+      r <- (div 1 powder)?;;
+      _ <- trigger (Syscall "print" [r]↑ top1);;
+      _ <- trigger (sPut (powder - 1)%Z↑);;
+      Ret r
+  .
+
+  Definition CannonSem: HModSem.t := {|
+    HModSem.fnsems := [("fire", cfunU fire_body)];
+    HModSem.initial_st := (1: Z)%Z↑;
+  |}
+  .
+
+  Definition Cannon: HMod.t := {|
+    HMod.get_modsem := fun _ => CannonSem;
+    HMod.sk := [("fire", Gfun↑)];
+  |}
+  .
+End CANNON.
