examples/cannon2/HCannon01proofH.v
@@ -1,0 +1,104 @@
+Require Import HoareDef STB HCannonRA HCannon0 HCannon1.
+Require Import Coqlib.
+Require Import ImpPrelude.
+Require Import Skeleton.
+Require Import PCM.
+Require Import ModSem Behavior.
+Require Import ProofMode.
+Require Import HPSim IProofMode.
+
+Set Implicit Arguments.
+
+
+
+Section SIMMODSEM.
+  Context `{Σ: GRA.t}.
+  Context `{@GRA.inG CannonRA Σ}.
+
+  Variable GlobalStb: Sk.t -> gname -> option fspec.
+  Variable o: ord.
+
+  (* state Invariant *)
+  Let Ist: Any.t -> Any.t -> iProp :=
+        fun st_src st_tgt => ((⌜st_src = (1: Z)↑ /\ st_tgt = (1: Z)↑⌝ ** OwnM (Ready))
+                                ∨ OwnM (Fired))%I
+  .
+
+  (* return relation *)
+  Let RR : (Any.t * Any.t) -> (Any.t * Any.t) -> iProp :=
+    fun '(st_src, ret_src) '(st_tgt, ret_tgt) => ⌜st_src = (1: Z)↑ /\ st_tgt = (1: Z)↑⌝ ** ⌜ret_src = ret_tgt⌝%I.
+
+  Theorem correct: IModPair.sim HCannon0.Cannon (HCannon1.Cannon GlobalStb o) Ist RR.
+  Proof.
+    econs; et. i. red.
+    econs; ss.
+    {
+      econs.
+      {
+        econs; ss. red. ii. iIntros. s.
+        unfold cfunU, cfunN, fire_body.
+        unfold HCannon0.fire_body at 2.
+        unfold sGet, sPut.
+        steps. ired_. steps. subst. unfold HCannon0.div in G1. 
+        ired_. unfold sGet. steps. grind.
+        assert ((1 `div` y2)%Z = 1). 
+         
+
+        
+      } 
+    }
+    { unfold Ist.  }
+
+  Theorem correct: refines2 [Cannon0.Cannon] [Cannon1.Cannon GlobalStb].
+  Proof.
+    (* proof using local simulation *)
+    eapply adequacy_local2. econs; ss. i. red.
+    econstructor 1 with (le:=le) (wf:=mk_wf wf); et; ss; cycle 1.
+
+    (* initial state *)
+    { exists tt. econs. eapply to_semantic.
+      iIntros "H". iLeft. iSplitR; ss. }
+
+    (* function "fire" *)
+    econs; ss. econs; ss. red.
+    (* use IPM *)
+    apply isim_fun_to_tgt; auto. i; ss.
+    (* state relation * precondition ⊢ isim (state relation* postcondition) p_src p_tgt *)
+    unfold Cannon0.fire_body, Cannon1.fire_body.
+    iIntros "[INV PRE]".
+    iDestruct "PRE" as "[[% BALL] %]". subst.
+    iEval (unfold inv_with, wf) in "INV".
+    iDestruct "INV" as (w1) "[[[% READY] | FIRED] _]".
+    { des; subst. hred_l. hred_r.
+      iApply isim_pget_tgt. hred_r.
+      iApply isim_syscall. iIntros (_).
+      hred_l. hred_r.
+      iApply isim_pput_tgt. hred_r.
+      iApply isim_ret. iSplit.
+      { iApply inv_with_current. iEval (unfold wf).
+        iRight. iCombine "READY" "BALL" as "FIRED".
+        iEval (rewrite <- ReadyBall). iApply "FIRED".
+      }
+      { iPureIntro. auto. }
+    }
+    { iCombine "FIRED" "BALL" as "FALSE".
+      iPoseProof (OwnM_valid with "FALSE") as "%".
+      exfalso. eapply FiredBall; auto.
+    }
+  Qed.
+
+  (* isim *)
+  (*   (* state relation *) *)
+  (*   le (* world future *) wf (* state relation *) w (* current world *) *)
+  (*   (* conditions for functions *) *)
+  (*   mn (* current module name *) conds (* conditions *) o (* maximal call depth (for termination) *) *)
+  (*   (* for coinduction *) *)
+  (*   (r, g, f_src, f_tgt) *)
+  (*   (* post condition : state_src -> state_tgt -> R_src -> R_tgt -> iProp *) *)
+  (*   Q *)
+  (*   (* source program : state_src * itree E R_src *) *)
+  (*   (st_src, prog_src) *)
+  (*   (* target program : state_tgt * itree E R_tgt*) *)
+  (*   (st_tgt, prog_tgt) *)
+
+End SIMMODSEM.
